riscv_model/spec/rsa_ops.dfy
@@ -37,4 +37,47 @@ module rsa_ops {
         to_nat_lemma_0(xs[..1]);
         reveal power();
     }
+
+    function seq_subb(xs: seq<uint32>, ys: seq<uint32>) : (seq<uint32>, uint1)
+        requires |xs| == |ys|
+        ensures var (zs, bout) := seq_subb(xs, ys);
+            && |zs| == |xs|
+    {
+        if |xs| == 0 then ([], 0)
+        else 
+            var len' := |xs| - 1;
+            var (zs, bin) := seq_subb(xs[..len'], ys[..len']);
+            var (z, bout) := uint32_subb(xs[len'], ys[len'], bin);
+            (zs + [z], bout)
+    }
+
+    lemma seq_subb_nat_lemma(xs: seq<uint32>, ys: seq<uint32>, zs: seq<uint32>, bout: uint1)
+        requires |xs| == |ys|
+        requires seq_subb(xs, ys) == (zs, bout);
+        ensures to_nat(xs) - to_nat(ys) + bout * pow_B32(|xs|) == to_nat(zs)
+    {
+        reveal to_nat();
+        if |xs| == 0 {
+            reveal power();
+        } else {
+            var len' := |xs| - 1;
+            var (zs', bin) := seq_subb(xs[..len'], ys[..len']);
+            var (z, _) := uint32_subb(xs[len'], ys[len'], bin);
+            assert bout * BASE_32 + xs[len'] - bin - ys[len'] == z;
+            
+            calc {
+                to_nat(zs);
+                to_nat(zs') + z * pow_B32(len');
+                    { seq_subb_nat_lemma(xs[..len'], ys[..len'], zs', bin); }
+                to_nat(xs[..len']) - to_nat(ys[..len']) + bin * pow_B32(len') + z * pow_B32(len');
+                to_nat(xs[..len']) - to_nat(ys[..len']) + xs[len'] * pow_B32(len')
+                    - ys[len'] * pow_B32(len') + bout * BASE_32 * pow_B32(len');
+                    { reveal to_nat(); }
+                to_nat(xs) - to_nat(ys) + bout * BASE_32 * pow_B32(len');
+                    { reveal power(); }
+                to_nat(xs) - to_nat(ys) + bout * pow_B32(|xs|);
+            }
+        }
+    }
+
 }
